poly_compress full proof WIP

proof/correctness/avx2/KyberPoly_avx2_prevec.ec
@@ -1,7 +1,7 @@
 require import AllCore List Int IntDiv CoreMap Real Number.
 from Jasmin require import JModel JMemory JWord.
-require import Array400 Array256 Array64 Array32 Array32p Array16 Array16p Array8 Array8p Array4 Array4p Array2p.
-require import WArray800 WArray512 WArray128 WArray128p WArray64 WArray32 WArray16.
+require import Array400 Array256 Array64 Array32 Array16 Array8 Array4 Array2p.
+require import WArray800 WArray512 WArray128 WArray128 WArray64 WArray32 WArray16.
 require W16extra.
 require import Fq.
 require import AVX2_Ops.
@@ -685,9 +685,9 @@ module Mavx2_prevec = {
     var t:t16u8;
     var i:int;
 
-    q <- Array16p.Array16.init (fun i => jqx16.[i]);
+    q <- Array16.init (fun i => jqx16.[i]);
 
-    shufbidx <- Array32p.Array32.init (fun i => pd_jshufbidx.[i]);
+    shufbidx <- Array32.init (fun i => pd_jshufbidx.[i]);
 
     mask_d <- Ops.iVPBROADCAST_8u32(pd_mask_s);
     mask <- f8u32_t16u16 mask_d;
@@ -715,145 +715,17 @@ module Mavx2_prevec = {
 
     return (rp);
   }
- 
- proc poly_decompress_restore (r:W16.t Array256.t) : W16.t Array256.t = {
-    var aux: int;
-    var rp: W16.t Array256.t;
-    var q: t16u16;
-    var shift: t16u16;
-    var f: t16u16;
-    var shift_d: t8u32;
-    var i: int;
 
-    q <- lift2poly(get256 (WArray32.init16 (fun i => jqx16.[i])) 0);
-    shift_d <- Ops.iVPBROADCAST_8u32(pd_shift_s);
-    shift <- f8u32_t16u16 shift_d;
-    aux <- (256 %/ 16);
-    i <- 0;
-
-    while (i < aux) {
-      f <- lift2poly(get256_direct (WArray512.init16 (fun i => r.[i])) (32 * i));
-
-      f <- Ops.iVPMULL_16u16(f, shift);
-      f <- Ops.iVPMULHRS_256(f, q);
-
-      rp <- fill (fun k => f.[k %% 16]) (16*i) 16 rp;
-      i <- i + 1;
-    }
-    return rp;
-  }
   (*--------------------------------------------------------------------*)
   proc poly_compress (rp:W64.t, a:W16.t Array256.t) : W16.t Array256.t = {
-    var aux: int;
-(*
-    var x16p:W16.t Array16.t;
-    var v:W256.t;
-    var shift1:W256.t;
-    var mask:W256.t;
-    var shift2:W256.t;
-    var permidx:W256.t;
-    var i:int;
-    var f0:W256.t;
-    var f1:W256.t;
-    var f2:W256.t;
-    var f3:W256.t;
-    x16p <- witness;
-    a <@ poly_csubq (a);
-    x16p <- jvx16;
-    v <- (get256 (WArray32.init16 (fun i => x16p.[i])) 0);
-    shift1 <- Ops.iVPBROADCAST_16u16(pc_shift1_s);
-    mask <- Ops.iVPBROADCAST_16u16(pc_mask_s);
-    shift2 <- Ops.iVPBROADCAST_16u16(pc_shift2_s);
-    permidx <- (get256 (WArray32.init32 (fun i => pc_permidx_s.[i])) 0);
-    aux <- (256 %/ 64);
-    i <- 0;
-    while (i < aux) {
-      f0 <- (get256 (WArray512.init16 (fun i => a.[i])) (4 * i));
-      f1 <- (get256 (WArray512.init16 (fun i => a.[i])) ((4 * i) + 1));
-      f2 <- (get256 (WArray512.init16 (fun i => a.[i])) ((4 * i) + 2));
-      f3 <- (get256 (WArray512.init16 (fun i => a.[i])) ((4 * i) + 3));
-      f0 <- Ops.iVPMULH_256(f0, v);
-      f1 <- Ops.iVPMULH_256(f1, v);
-      f2 <- Ops.iVPMULH_256(f2, v);
-      f3 <- Ops.iVPMULH_256(f3, v);
-      f0 <- Ops.iVPMULHRS_256(f0, shift1);
-      f1 <- Ops.iVPMULHRS_256(f1, shift1);
-      f2 <- Ops.iVPMULHRS_256(f2, shift1);
-      f3 <- Ops.iVPMULHRS_256(f3, shift1);
-      f0 <- Ops.ivpand16u16(f0, mask);
-      f1 <- Ops.ivpand16u16(f1, mask);
-      f2 <- Ops.ivpand16u16(f2, mask);
-      f3 <- Ops.ivpand16u16(f3, mask);
-      f0 <- Ops.iVPACKUS_16u16(f0, f1);
-      f2 <- Ops.iVPACKUS_16u16(f2, f3);
-      f0 <- Ops.iVPMADDUBSW_256(f0, shift2);
-      f2 <- Ops.iVPMADDUBSW_256(f2, shift2);
-      f0 <- Ops.iVPACKUS_16u16(f0, f2);
-      f0 <- Ops.iVPERMD(permidx, f0);
-      Glob.mem <-
-      storeW256 Glob.mem (W64.to_uint (rp + (W64.of_int (32 * i)))) f0;
-      i <- i + 1;
-    }
-*)
-    return (a);
-  }
-
-  proc poly_compress_round (a:W16.t Array256.t) : W16.t Array256.t = {
-    var rp: W16.t Array256.t;
     var aux: int;
 
     var v: t16u16;
     var shift1: t16u16;
     var mask: t16u16;
-    var i: int;
-    var f0: t16u16;
-    var f1: t16u16;
-    var f2: t16u16;
-    var f3: t16u16;
-
-    a <@ poly_csubq (a);
-
-    v <- lift2poly(get256 (WArray32.init16 (fun i => jvx16.[i])) 0);
-    shift1 <- Ops.iVPBROADCAST_16u16(pc_shift1_s);
-    mask <- Ops.iVPBROADCAST_16u16(pc_mask_s);
-    aux <- (256 %/ 64);
-    i <- 0;
-
-    while (i < aux) {
-      f0 <- lift2poly (get256 (WArray512.init16 (fun i => a.[i])) (4 * i));
-      f1 <- lift2poly (get256 (WArray512.init16 (fun i => a.[i])) ((4 * i) + 1));
-      f2 <- lift2poly (get256 (WArray512.init16 (fun i => a.[i])) ((4 * i) + 2));
-      f3 <- lift2poly (get256 (WArray512.init16 (fun i => a.[i])) ((4 * i) + 3));
-
-      f0 <- Ops.iVPMULH_256(f0, v);
-      f1 <- Ops.iVPMULH_256(f1, v);
-      f2 <- Ops.iVPMULH_256(f2, v);
-      f3 <- Ops.iVPMULH_256(f3, v);
-      f0 <- Ops.iVPMULHRS_256(f0, shift1);
-      f1 <- Ops.iVPMULHRS_256(f1, shift1);
-      f2 <- Ops.iVPMULHRS_256(f2, shift1);
-      f3 <- Ops.iVPMULHRS_256(f3, shift1);
-      f0 <- Ops.ivpand16u16(f0, mask);
-      f1 <- Ops.ivpand16u16(f1, mask);
-      f2 <- Ops.ivpand16u16(f2, mask);
-      f3 <- Ops.ivpand16u16(f3, mask);
-
-      rp <- fill (fun k => f0.[k %% 16]) (64*i) 16 rp;
-      rp <- fill (fun k => f1.[k %% 16]) (64*i + 16) 16 rp;
-      rp <- fill (fun k => f2.[k %% 16]) (64*i + 32) 16 rp;
-      rp <- fill (fun k => f3.[k %% 16]) (64*i + 48) 16 rp;
-
-      i <- i + 1;
-    }
-    return rp;
-  }
-
-  proc poly_compress_store (rp:W64.t, a:W16.t Array256.t) : unit = {
-    var aux: int;
-
     var shift2: t16u16;
     var permidx: t8u32;
-    var i:int;
+    var i: int;
     var f0: t16u16;
     var f1: t16u16;
     var f2: t16u16;
@@ -864,34 +736,51 @@ module Mavx2_prevec = {
     var f2_b: t32u8;
     var shift2_b: t32u8;
 
+
     a <@ poly_csubq (a);
 
+    v <- Array16.init (fun i => jvx16.[i]);
+    shift1 <- Ops.iVPBROADCAST_16u16(pc_shift1_s);
+    mask <- Ops.iVPBROADCAST_16u16(pc_mask_s);
     shift2 <- Ops.iVPBROADCAST_16u16(pc_shift2_s);
-    shift2_b <- f16u16_t32u8 shift2;
-    (* permidx <- (get256 (WArray32.init32 (fun i => pc_permidx_s.[i])) 0); *)
+    shift2_b <- f16u16_t32u8 shift2; (* FIXME: specific AVX2 op maybe ?? *)
+    permidx <- Array8.init (fun i => pc_permidx_s.[i]);
+
     aux <- (256 %/ 64);
     i <- 0;
 
     while (i < aux) {
-      f0 <- lift2poly (get256 (WArray512.init16 (fun i => a.[i])) (4 * i));
-      f1 <- lift2poly (get256 (WArray512.init16 (fun i => a.[i])) ((4 * i) + 1));
-      f2 <- lift2poly (get256 (WArray512.init16 (fun i => a.[i])) ((4 * i) + 2));
-      f3 <- lift2poly (get256 (WArray512.init16 (fun i => a.[i])) ((4 * i) + 3));
+      f0 <- Array16.init (fun j => a.[64*i+j]);
+      f1 <- Array16.init (fun j => a.[64*i+16+j]);
+      f2 <- Array16.init (fun j => a.[64*i+32+j]);
+      f3 <- Array16.init (fun j => a.[64*i+48+j]);
+      f0 <- Ops.iVPMULH_256(f0, v);
+      f1 <- Ops.iVPMULH_256(f1, v);
+      f2 <- Ops.iVPMULH_256(f2, v);
+      f3 <- Ops.iVPMULH_256(f3, v);
+      f0 <- Ops.iVPMULHRS_256(f0, shift1);
+      f1 <- Ops.iVPMULHRS_256(f1, shift1);
+      f2 <- Ops.iVPMULHRS_256(f2, shift1);
+      f3 <- Ops.iVPMULHRS_256(f3, shift1);
+      f0 <- Ops.ivpand16u16(f0, mask);
+      f1 <- Ops.ivpand16u16(f1, mask);
+      f2 <- Ops.ivpand16u16(f2, mask);
+      f3 <- Ops.ivpand16u16(f3, mask);
 
       f0_b <- Ops.iVPACKUS_16u16(f0, f1);
       f2_b <- Ops.iVPACKUS_16u16(f2, f3);
       f0 <- Ops.iVPMADDUBSW_256(f0_b, shift2_b);
       f2 <- Ops.iVPMADDUBSW_256(f2_b, shift2_b);
       f0_b <- Ops.iVPACKUS_16u16(f0, f2);
+
       f0_dw <- f32u8_t8u32 f0_b;
-      (* f0_dw <- Ops.iVPERMD(permidx, f0_dw); *)
+      f0_dw <- Ops.iVPERMD(permidx, f0_dw);  (* FIXME: specific AVX2 op maybe ?? *)
       f0_b <- f8u32_t32u8 f0_dw;
 
       Glob.mem <- Ops.istore32u8(Glob.mem, rp + (W64.of_int (32 * i)), f0_b);
-
       i <- i + 1;
     }
+
+    return (a);
   }
-
-
 }.
